Batteries/Data/Fin/Fold.lean
@@ -4,8 +4,212 @@ Released under Apache 2.0 license as described in the file LICENSE.
 Authors: François G. Dorais
 -/
 import Batteries.Data.List.FinRange
+import Batteries.Data.Fin.Basic
 
 namespace Fin
+
+/-! ### dfoldlM -/
+
+theorem dfoldlM_loop_lt [Monad m] {n : Nat} {α : Fin (n+1) → Type _}
+    (f : ∀ (i : Fin n), α i.castSucc → m (α i.succ))
+    (h : i < n) (x : α ⟨i, Nat.lt_add_right 1 h⟩) :
+      dfoldlM.loop n α f i (Nat.lt_add_right 1 h) x =
+        (f ⟨i, h⟩ x) >>= (dfoldlM.loop n α f (i+1) (Nat.add_lt_add_right h 1)) := by
+  rw [dfoldlM.loop, dif_pos h]
+
+theorem dfoldlM_loop_eq [Monad m] {n : Nat} {α : Fin (n+1) → Type _}
+    (f : ∀ (i : Fin n), α i.castSucc → m (α i.succ)) (x : α ⟨n, Nat.le_refl _⟩) :
+      dfoldlM.loop n α f n (Nat.le_refl _) x = pure x := by
+  rw [dfoldlM.loop, dif_neg (Nat.lt_irrefl _), cast_eq]
+
+@[simp] theorem dfoldlM_zero [Monad m] {α : Fin 1 → Type _}
+    (f : (i : Fin 0) → α i.castSucc → m (α i.succ)) (x : α 0) :
+      dfoldlM 0 α f x = pure x :=
+  dfoldlM_loop_eq ..
+
+theorem dfoldlM_loop [Monad m] {n : Nat} {α : Fin (n+2) → Type _}
+    (f : (i : Fin (n+1)) → α i.castSucc → m (α i.succ))
+    (h : i < n+1) (x : α ⟨i, Nat.lt_add_right 1 h⟩) :
+      dfoldlM.loop (n+1) α f i (Nat.lt_add_right 1 h) x =
+        f ⟨i, h⟩ x >>= (dfoldlM.loop n (α ∘ succ) (f ·.succ ·) i h .) := by
+  if h' : i < n then
+    rw [dfoldlM_loop_lt _ h _]
+    congr; funext
+    rw [dfoldlM_loop_lt _ h' _, dfoldlM_loop]; rfl
+  else
+    cases Nat.le_antisymm (Nat.le_of_lt_succ h) (Nat.not_lt.1 h')
+    rw [dfoldlM_loop_lt]
+    congr; funext
+    rw [dfoldlM_loop_eq, dfoldlM_loop_eq]
+
+theorem dfoldlM_succ [Monad m] {n : Nat} {α : Fin (n+2) → Type _}
+    (f : (i : Fin (n+1)) → α i.castSucc → m (α i.succ)) (x : α 0) :
+      dfoldlM (n+1) α f x = f 0 x >>= (dfoldlM n (α ∘ succ) (f ·.succ ·) .) :=
+  dfoldlM_loop ..
+
+/-- Dependent version `dfoldlM` equals non-dependent version `foldlM` -/
+theorem dfoldlM_eq_foldlM [Monad m] {n : Nat} {α : Type _} (f : (i : Fin n) → α → m α) (x : α) :
+    dfoldlM n (fun _ => α) f x = foldlM n (fun x i => f i x) x := by
+  induction n generalizing x with
+  | zero => simp only [dfoldlM_zero, foldlM_zero]
+  | succ n ih =>
+    simp only [dfoldlM_succ, foldlM_succ, Function.comp_apply, Function.comp_def]
+    congr; ext; simp only [ih]
+
+/-! ### dfoldrM -/
+
+theorem dfoldrM_loop_zero [Monad m] {n : Nat} {α : Fin (n+1) → Type _}
+    (f : (i : Fin n) → α i.succ → m (α i.castSucc)) (x : α 0) :
+      dfoldrM.loop n α f 0 (Nat.zero_lt_succ n) x = pure x := by
+  rw [dfoldrM.loop, dif_neg (Nat.not_lt_zero _), cast_eq]
+
+theorem dfoldrM_loop_succ [Monad m] {n : Nat} {α : Fin (n+1) → Type _}
+    (f : (i : Fin n) → α i.succ → m (α i.castSucc)) (h : i < n)
+    (x : α ⟨i+1, Nat.add_lt_add_right h 1⟩) :
+      dfoldrM.loop n α f (i+1) (Nat.add_lt_add_right h 1) x =
+        f ⟨i, h⟩ x >>= dfoldrM.loop n α f i (Nat.lt_add_right 1 h) := by
+  rw [dfoldrM.loop, dif_pos (Nat.zero_lt_succ i)]
+  simp only [Nat.add_one_sub_one, castSucc_mk, succ_mk, eq_mpr_eq_cast, cast_eq]
+
+theorem dfoldrM_loop [Monad m] [LawfulMonad m] {n : Nat} {α : Fin (n+2) → Type _}
+    (f : (i : Fin (n+1)) → α i.succ → m (α i.castSucc)) (h : i+1 ≤ n+1)
+    (x : α ⟨i+1, Nat.add_lt_add_right h 1⟩) :
+      dfoldrM.loop (n+1) α f (i+1) (Nat.add_lt_add_right h 1) x =
+        dfoldrM.loop n (α ∘ succ) (f ·.succ) i h x >>= f 0 := by
+  induction i with
+  | zero =>
+    rw [dfoldrM_loop_zero, dfoldrM_loop_succ, pure_bind]
+    conv => rhs; rw [←bind_pure (f 0 x)]
+    congr; funext; exact dfoldrM_loop_zero ..
+  | succ i ih =>
+    rw [dfoldrM_loop_succ _ h, dfoldrM_loop_succ _ (Nat.succ_lt_succ_iff.mp h), bind_assoc]
+    congr; funext; exact ih ..
+
+@[simp] theorem dfoldrM_zero [Monad m] {α : Fin 1 → Type _}
+    (f : (i : Fin 0) → α i.succ → m (α i.castSucc)) (x : α 0) :
+      dfoldrM 0 α f x = pure x :=
+  dfoldrM_loop_zero ..
+
+theorem dfoldrM_succ [Monad m] [LawfulMonad m] {n : Nat} {α : Fin (n+2) → Type _}
+    (f : (i : Fin (n+1)) → α i.succ → m (α i.castSucc)) (x : α (last (n+1))) :
+      dfoldrM (n+1) α f x = dfoldrM n (α ∘ succ) (f ·.succ) x >>= f 0 :=
+  dfoldrM_loop ..
+
+/-- Dependent version `dfoldrM` equals non-dependent version `foldrM` -/
+theorem dfoldrM_eq_foldrM [Monad m] [LawfulMonad m] {n : Nat} {α : Type _}
+    (f : (i : Fin n) → α → m α) (x : α) : dfoldrM n (fun _ => α) f x = foldrM n f x := by
+  induction n generalizing x with
+  | zero => simp only [dfoldrM_zero, foldrM_zero]
+  | succ n ih => simp only [dfoldrM_succ, foldrM_succ, Function.comp_def, ih]
+
+/-! ### dfoldl -/
+
+theorem dfoldl_loop_lt {n : Nat} {α : Fin (n+1) → Sort _}
+    (f : ∀ (i : Fin n), α i.castSucc → α i.succ) (h : i < n) (x : α ⟨i, Nat.lt_add_right 1 h⟩) :
+      dfoldl.loop n α f i (Nat.lt_add_right 1 h) x =
+        dfoldl.loop n α f (i+1) (Nat.add_lt_add_right h 1) (f ⟨i, h⟩ x) := by
+  rw [dfoldl.loop, dif_pos h]
+
+theorem dfoldl_loop_eq {n : Nat} {α : Fin (n+1) → Sort _}
+    (f : ∀ (i : Fin n), α i.castSucc → α i.succ) (x : α ⟨n, Nat.le_refl _⟩) :
+      dfoldl.loop n α f n (Nat.le_refl _) x = x := by
+  rw [dfoldl.loop, dif_neg (Nat.lt_irrefl _), cast_eq]
+
+@[simp] theorem dfoldl_zero {α : Fin 1 → Sort _} (f : (i : Fin 0) → α i.castSucc → α i.succ)
+    (x : α 0) : dfoldl 0 α f x = x :=
+  dfoldl_loop_eq ..
+
+theorem dfoldl_loop {n : Nat} {α : Fin (n+2) → Sort _}
+    (f : (i : Fin (n+1)) → α i.castSucc → α i.succ) (h : i < n+1)
+    (x : α ⟨i, Nat.lt_add_right 1 h⟩) :
+      dfoldl.loop (n+1) α f i (Nat.lt_add_right 1 h) x =
+        dfoldl.loop n (α ∘ succ) (f ·.succ ·) i h (f ⟨i, h⟩ x) := by
+  if h' : i < n then
+    rw [dfoldl_loop_lt _ h _]
+    rw [dfoldl_loop_lt _ h' _, dfoldl_loop]; rfl
+  else
+    cases Nat.le_antisymm (Nat.le_of_lt_succ h) (Nat.not_lt.1 h')
+    rw [dfoldl_loop_lt]
+    rw [dfoldl_loop_eq, dfoldl_loop_eq]
+
+theorem dfoldl_succ {n : Nat} {α : Fin (n+2) → Sort _}
+    (f : (i : Fin (n+1)) → α i.castSucc → α i.succ) (x : α 0) :
+      dfoldl (n+1) α f x = dfoldl n (α ∘ succ) (f ·.succ ·) (f 0 x) :=
+  dfoldl_loop ..
+
+theorem dfoldl_succ_last {n : Nat} {α : Fin (n+2) → Sort _}
+    (f : (i : Fin (n+1)) → α i.castSucc → α i.succ) (x : α 0) :
+      dfoldl (n+1) α f x = f (last n) (dfoldl n (α ∘ castSucc) (f ·.castSucc ·) x) := by
+  rw [dfoldl_succ]
+  induction n with
+  | zero => simp [dfoldl_succ, last]
+  | succ n ih => rw [dfoldl_succ, @ih (α ∘ succ) (f ·.succ ·), dfoldl_succ]; congr
+
+/-- Dependent version `dfoldl` equals non-dependent version `foldl` -/
+theorem dfoldl_eq_foldl {α : Sort _} (f : Fin n → α → α) (x : α) :
+    dfoldl n (fun _ => α) f x = foldl n (fun x i => f i x) x := by
+  induction n generalizing x with
+  | zero => simp only [dfoldl_zero, foldl_zero]
+  | succ n ih =>
+    simp only [dfoldl_succ, foldl_succ, Function.comp_apply, Function.comp_def]
+    congr; simp only [ih]
+
+/-! ### dfoldr -/
+
+theorem dfoldr_loop_zero {n : Nat} {α : Fin (n+1) → Sort _}
+    (f : (i : Fin n) → α i.succ → α i.castSucc) (x : α 0) :
+      dfoldr.loop n α f 0 (Nat.zero_lt_succ n) x = x := by
+  rw [dfoldr.loop, dif_neg (Nat.not_lt_zero _), cast_eq]
+
+theorem dfoldr_loop_succ {n : Nat} {α : Fin (n+1) → Sort _}
+    (f : (i : Fin n) → α i.succ → α i.castSucc) (h : i < n)
+    (x : α ⟨i+1, Nat.add_lt_add_right h 1⟩) :
+      dfoldr.loop n α f (i+1) (Nat.add_lt_add_right h 1) x =
+        dfoldr.loop n α f i (Nat.lt_add_right 1 h) (f ⟨i, h⟩ x) := by
+  rw [dfoldr.loop, dif_pos (Nat.zero_lt_succ i)]
+  simp only [Nat.add_one_sub_one, succ_mk, eq_mpr_eq_cast, cast_eq]
+
+theorem dfoldr_loop {n : Nat} {α : Fin (n+2) → Sort _}
+    (f : (i : Fin (n+1)) → α i.succ → α i.castSucc) (h : i+1 ≤ n+1)
+    (x : α ⟨i+1, Nat.add_lt_add_right h 1⟩) :
+      dfoldr.loop (n+1) α f (i+1) (Nat.add_lt_add_right h 1) x =
+        f 0 (dfoldr.loop n (α ∘ succ) (f ·.succ) i h x) := by
+  induction i with
+  | zero => simp [dfoldr_loop_succ, dfoldr_loop_zero]
+  | succ i ih => rw [dfoldr_loop_succ _ h, dfoldr_loop_succ _ (Nat.succ_lt_succ_iff.mp h),
+      ih (Nat.le_of_succ_le h)]; rfl
+
+@[simp] theorem dfoldr_zero {α : Fin 1 → Sort _} (f : (i : Fin 0) → α i.succ → α i.castSucc)
+    (x : α 0) : dfoldr 0 α f x = x :=
+  dfoldr_loop_zero ..
+
+theorem dfoldr_succ {n : Nat} {α : Fin (n+2) → Sort _}
+    (f : (i : Fin (n+1)) → α i.succ → α i.castSucc) (x : α (last (n+1))) :
+      dfoldr (n+1) α f x = f 0 (dfoldr n (α ∘ succ) (f ·.succ) x) :=
+  dfoldr_loop ..
+
+theorem dfoldr_succ_last {n : Nat} {α : Fin (n+2) → Sort _}
+    (f : (i : Fin (n+1)) → α i.succ → α i.castSucc) (x : α (last (n+1))) :
+      dfoldr (n+1) α f x = dfoldr n (α ∘ castSucc) (f ·.castSucc) (f (last n) x) := by
+  induction n with
+  | zero => simp only [dfoldr_succ, dfoldr_zero, last, zero_eta]
+  | succ n ih => rw [dfoldr_succ, ih (α := α ∘ succ) (f ·.succ), dfoldr_succ]; congr
+
+theorem dfoldr_eq_dfoldrM {n : Nat} {α : Fin (n+1) → Type _}
+    (f : (i : Fin n) → α i.succ → α i.castSucc) (x : α (last n)) :
+      dfoldr n α f x = dfoldrM (m:=Id) n α f x := by
+  induction n <;> simp [dfoldr_succ, dfoldrM_succ, *]
+
+/-- Dependent version `dfoldr` equals non-dependent version `foldr` -/
+theorem dfoldr_eq_foldr {n : Nat} {α : Sort _} (f : Fin n → α → α) (x : α) :
+    dfoldr n (fun _ => α) f x = foldr n f x := by
+  induction n with
+  | zero => simp only [dfoldr_zero, foldr_zero]
+  | succ n ih => simp only [dfoldr_succ, foldr_succ, Function.comp_apply, Function.comp_def, ih]
+
+-- TODO: add `dfoldl_rev` and `dfoldr_rev`
+
+/-! ### `Fin.fold{l/r}{M}` equals `List.fold{l/r}{M}` -/
 
 theorem foldlM_eq_foldlM_finRange [Monad m] (f : α → Fin n → m α) (x) :
     foldlM n f x = (List.finRange n).foldlM f x := by
